\documentclass{article}
\author{xuyou}
\title{Proof For Prop 1 and 2 in GraphWave}
\usepackage{xeCJK}
\usepackage{bm}
\begin{document}
\maketitle
\section{note for prop 1} 
\subsection{equation 1}
\begin{center}
\[
\sum _ { m=1  }^N\left( \Psi _ { m a } ^ { ( s ) } \right) ^ { 2 }
=\Psi_{aa}^{(2s)}
\]
\end{center}
because left side equal \bm{$1_a^T$}$Ug(s\Lambda)g(s\Lambda)U^T$\bm{$1_a$}=
$\Psi_{aa}^{(2s)}$
\subsection{equation 2}
\begin{center}

\[
\sum_{m=1}^N \Psi_{ma}^{(s)}=1 \quad s\ for\ any\ value
\]
\end{center}
%\paragraph{}
because 1 is the eigenvalue of $\Psi^{(s)}$ for eigenvector \textbf{1}
\section{note for prop 2} 
$\Psi^s$ eigenvector for eigenvalue 1
\begin{center}
$U_{.1}=\frac{1}{\sqrt{N}}$
\end{center}
so\begin{center}
$\left|\Psi_{aa}^{(s+1)}-\frac{1}{N}\right|=\left|\sum_{j=1}^Ne^{-\lambda_j(s+1)}U_{ja}^2-\frac{1}{N}\right|=\left| \sum _ { j = 2 } ^ { N } e ^ { - \lambda _ { j } ( s + 1 ) } U _ { j a } ^ { 2 } \right|\leq
\left| \sum _ { j = 2 } ^ { N }e^{\lambda_2s} e ^ { - \lambda _ { j } s  } U _ { j a } ^ { 2 } \right|=e ^ { - \lambda _ { 2 } } \left| \Psi _ { a a } ^ { ( s ) } - \frac { 1 } { N } \right|$

\end{center} 
\end{document}